WIP: working on label prop invar

dataplane/Examples/Label_Propagation_op_Correctness.thy
@@ -139,32 +139,6 @@ value [GHC] \<open>ltaken 2 (lmap show_Outs (trace_exec (compiled test_input9)))
 *)
 
 
-context
-  fixes edges :: \<open>('a \<times> 'a) set\<close> (\<open>E\<close>)
-begin
-
-(* Undirected reachability and connected components *)
-
-definition reachable where
-  \<open>reachable x y \<equiv> (x, y) \<in> (E \<union> E\<inverse>)\<^sup>*\<close>
-
-definition is_subcc :: \<open>'a set \<Rightarrow> bool\<close>  where
-  \<open>is_subcc S \<equiv> \<forall>x \<in> S. \<forall>y \<in> S. reachable x y\<close>
-
-definition is_cc :: \<open>'a set \<Rightarrow> bool\<close> where
-  \<open>is_cc S \<equiv> S \<noteq> {} \<and> is_subcc S \<and> (\<forall>S'. S \<subseteq> S' \<and> is_subcc S' \<longrightarrow> S' = S)\<close>
-
-abbreviation ccs :: \<open>'a set set\<close> where
-  \<open>ccs \<equiv> {S. is_cc S}\<close>
-
-definition is_ccs :: \<open>'a set set \<Rightarrow> bool\<close> where
-  \<open>is_ccs \<equiv> (=) ccs\<close>
-
-lemma Ex1_is_ccs:
-  \<open>Ex1 is_ccs\<close>
-  unfolding is_ccs_def by blast
-
-end
 
 definition \<open>raw_summary = (\<lambda>l1 l2. case (find (\<lambda> (l1', s, l2'). l1' = l1 \<and> l2 = l2')
   [(Loc 0 (Trg 0), [MyPair 0 0], Loc 0 (Src 0)), (Loc 0 (Trg 1), [MyPair 0 0], Loc 0 (Src 1)), (Loc 0 (Src 0), [MyPair 0 0], Loc 1 (Trg 0)), (Loc 1 (Trg 0), [MyPair 0 0], Loc 1 (Src 0)),
@@ -268,6 +242,44 @@ lemma Inr_2_1_in_ran[simp]:
 
 find_consts "_ list \<Rightarrow> _ cset"
 
+
+context
+  fixes edges :: \<open>('a \<times> 'a) set\<close> (\<open>E\<close>)
+begin
+
+(* Undirected reachability and connected components *)
+
+definition reachable where
+  \<open>reachable x y \<equiv> (x, y) \<in> (E \<union> E\<inverse>)\<^sup>*\<close>
+
+definition is_subcc :: \<open>'a set \<Rightarrow> bool\<close>  where
+  \<open>is_subcc S \<equiv> \<forall>x \<in> S. \<forall>y \<in> S. reachable x y\<close>
+
+definition is_cc :: \<open>'a set \<Rightarrow> bool\<close> where
+  \<open>is_cc S \<equiv> S \<noteq> {} \<and> is_subcc S \<and> (\<forall>S'. S \<subseteq> S' \<and> is_subcc S' \<longrightarrow> S' = S)\<close>
+
+abbreviation ccs :: \<open>'a set set\<close> where
+  \<open>ccs \<equiv> {S. is_cc S}\<close>
+
+definition is_ccs :: \<open>'a set set \<Rightarrow> bool\<close> where
+  \<open>is_ccs \<equiv> (=) ccs\<close>
+
+lemma Ex1_is_ccs:
+  \<open>Ex1 is_ccs\<close>
+  unfolding is_ccs_def by blast
+
+definition cc_of where
+  "cc_of v = {u. reachable v u}"
+
+definition labels_inv  where
+  "labels_inv l \<longleftrightarrow> (\<forall>v. l v \<in> cc_of v)"
+
+end
+
+term labels_inv
+term "label os_label_prop"
+
+
 lemma label_propagation_correctness:
   fixes lxs :: \<open>((nat, nat) myprod, nat \<times> nat) event llist\<close>
     and os :: \<open>3 \<Rightarrow> (2, nat \<times> nat + nat set set, (nat, nat) myprod) operator_state\<close>
@@ -305,13 +317,16 @@ lemma label_propagation_correctness:
     \<open>SO = cset_from_list (map (\<lambda>x. ((1, 0), x)) (outpu (os 1) 0))\<close>
     and input_stream_inv:
     \<open>timely_input_stream lxs (mset (ocaps (os 0) 0))\<close>
+    and label_prop_inv:
+    \<open>(\<forall> t \<in> set (timestamps os_label_prop). labels_inv (all_edges os_label_prop t) (label os_label_prop t))\<close>
   shows \<open>set_op S D (dataflow_op sg (G_op os_input os_label_prop (os 2) cbufs))
          \<approx> set_spec_op (cUn (cUn S SO) SP) D\<close>
   using assms
 proof (coinduction arbitrary: S SO SP D lxs os os_input os_label_prop cbufs chns sg T G V L
     rule: weakBisimWeakUptoBisimCong)
   case SIM1
-  note subgraph_inv = SIM1(1,2)
+  note subgraph_inv = SIM1(1,2) 
+  and label_prop_inv = SIM1(16)
   show ?case (is \<open>wsim ((~) OO \<U> ?R OO (\<approx>)) _ _\<close>)
   proof -
     thm SIM1
@@ -454,9 +469,18 @@ proof (coinduction arbitrary: S SO SP D lxs os os_input os_label_prop cbufs chns
                             subgoal
                             apply simp
                           apply (clarsimp split: list.splits)
-                          subgoal for a as
+                              subgoal for a as
+                                apply safe
+                                subgoal for X
+                                  unfolding is_cc_def is_subcc_def
+                                  apply (intro conjI ballI)
+                                  subgoal
+                                    sorry
+                                  subgoal for x y
+                                apply (drule label_prop_inv[unfolded SIM1(6) operator_state.defs, simplified, rule_format, of "myfst t'"])
+                                unfolding labels_inv_def
 
-                      find_theorems "coll _ _ = _"
+                      find_theorems os_label_prop
 
 end
                   apply (simp only: cUn_assoc cimage_cUn)
